FStar.DM4F.IFC.fst

examples/dm4free/FStar.DM4F.IFC.fst
@@ -4,66 +4,23 @@ module FStar.DM4F.IFC
 (* Effect (ifc a) : A monad for dynamic information-flow control                *)
 (********************************************************************************)
 
-(* TODO: This has not been whitelisted
 type label =
   | Low
   | High
-*)
-type label = bool
-let low = true
-let high = false
-
-let join l1 l2 =
-    if l1 = high || l2 = high then high else low
-
-let flows l1 l2 = not(l1=high && l2=low)
 
 let ifc (a:Type) = label -> M (option (a * label))
 
-(* open FStar.FunctionalExtensionality *)
-
-(* let eq_ifc (a:Type) (f:ifc a) (g:ifc a) = *)
-(*    forall l. f l == g l *)
-
 let return_ifc (a:Type) (x:a) : ifc a = fun l -> Some (x, l)
 let bind_ifc (a:Type) (b:Type) (f:ifc a) (g: a -> Tot (ifc b)) : ifc b
-  = fun l0 -> let fl0 = f l0 in match fl0 with
-           | None -> None
-           | Some (x, l1) ->
-             let gxl1 = g x l1 in match gxl1 with
-             | None -> None
-             | Some (y, l2) -> Some(y, l2)
+  = fun l0 -> let fl0 = f l0 in
+              match fl0 with
+              | None -> None
+              | Some (x, l1) ->
+                let gxl1 = g x l1 in
+                match gxl1 with
+                | None -> None
+                | Some (y, l2) -> Some(y, l2)
 
-(* val left_unit: a:Type -> b:Type -> x:a -> f:(a -> Tot (ifc b)) *)
-(*             -> Lemma (eq_ifc b (bind_ifc a b (return_ifc a x) f) (f x)) *)
-(* let left_unit a b x f = admit() (\* #710 *\) *)
-
-(* val right_unit: a:Type -> f:ifc a -> Lemma (eq_ifc a (bind_ifc a a f (return_ifc a)) f) *)
-(* let right_unit a f = admit() (\* #710 *\) *)
-
-(* val associativity: a:Type -> b:Type -> c:Type -> f:ifc a -> g:(a -> Tot (ifc b)) -> h:(b -> Tot (ifc c)) *)
-(*                  -> Lemma (eq_ifc c (bind_ifc a c f (fun x -> bind_ifc b c (g x) h)) (bind_ifc b c (bind_ifc a b f g) h)) *)
-(* let associativity a b c f g h = () *)
-
-
-
-(* // A sample monadic program (normally would write this after *)
-(* // elaboration, but whatever, can write this in DM too) *)
-(* val p : unit -> Pure (ifc unit) (requires True) (ensures (fun r -> forall l. r l = None)) *)
-(* (\* Weak type (works): unit -> Tot (ifc unit) *\) *)
-(* (\* Alternative strong type (doesn't work), (Valid(ApplyTT@2 @0)) *)
-(*   unit -> Tot (label -> Pure (err (unit * label)) (requires True) (ensures (fun r -> r = None))) *\) *)
-(* (\* let p () = bind_ifc _ _ (read low)              (fun b1 -> *\) *)
-(* (\*            bind_ifc _ _ (read low)              (fun b2 -> *\) *)
-(* (\*            bind_ifc _ _ (write low (b1 && b2))  (fun _  -> *\) *)
-(* (\*            bind_ifc _ _ (read high)             (fun b3 -> *\) *)
-(* (\*            bind_ifc _ _ (write high (b1 || b3)) (fun _  -> *\) *)
-(* (\*                         (write low (xor b3 b3))  ))))) *\) *)
-(* let p () = admit() (\* #710 *\) *)
-
-(* TODO: without reifiable, this fails weirdly. Cf #709 *)
-
-//#set-options "--debug FStar.DM4F.IFC --debug_level ED --debug_level Extreme --print_implicits --print_bound_var_types --log_queries"
 reifiable new_effect_for_free {
   IFC : a:Type -> Effect
   with
@@ -80,27 +37,28 @@ inline let lift_pure_exnst (a:Type) (wp:pure_wp a) (h0:label) (p:IFC.post a) =
   wp (fun a -> p (Some (a, h0)))
 sub_effect PURE ~> IFC = lift_pure_exnst
 
-assume val read : l:label -> IFC bool (fun l0 p -> forall b. p (Some (b, join l0 l)))
-assume val write : l:label -> bool -> IFC unit (fun l0 p -> if flows l0 l then p (Some ((), l0)) else  p None)
+// read and write are assumed, since we don't model I/O precisely here
+
+let join l1 l2 = if l1 = High || l2 = High then High else Low
+
+let flows l1 l2 = not(l1=High && l2=Low)
+
+assume val read : l:label -> IFC bool
+  (fun l0 p -> forall b. p (Some (b, join l0 l)))
+
+assume val write : l:label -> bool -> IFC unit
+  (fun l0 p -> if flows l0 l then p (Some ((), l0)) else p None)
+
+// A simple program using the IFC effect
+
 let xor (b1:bool) (b2:bool) : Tot bool = not (b1 = b2)
 
-val p' : unit ->  Ifc unit (requires (fun l   -> True))
+val p : unit ->  Ifc unit (requires (fun l   -> True))
                           (ensures  (fun l r -> r = None))
-let p' () =
-  let b1 = read low in
-  let b2 = read low in
-  write low (b1 && b2);
-  let b3 = read high in
-  write high (b1 || b3);
-  write low (xor b3 b3)
-
-(* (\* just a sanity check for Guido: this works with the pure to Ifc coercion; *)
-(*    btw. can't we get the pure to X coercion for free too ?*\) *)
-(* val p'' : unit -> Ifc unit (requires (fun l   -> True)) *)
-(*                            (ensures  (fun l r -> True)) *)
-(* let p'' () = () *)
-
-(* (\* [8:14:57 PM] Nik Swamy: I think for bonus points, in the ifc monad we could *\) *)
-(* (\* [8:15:33 PM] Nik Swamy: 1. add outputs, a list of Booleans, e.g., and have the write cons to it *\) *)
-(* (\* [8:15:48 PM] Nik Swamy: 2. add an input state so that read is not a constant *\) *)
-(* (\* [8:16:23 PM] Nik Swamy: 3. do a relational proof of the p program showing that despite the exception, the outputs would be the same in 2 runs *\) *)
+let p () =
+  let b1 = read Low in
+  let b2 = read Low in
+  write Low (b1 && b2);
+  let b3 = read High in
+  write High (b1 || b3);
+  write Low (xor b3 b3)
